Introduce equiv_env to factorize the equivalence between Lustre and Imp memories

Correctness.v
@@ -367,12 +367,38 @@ Local Ltac split_env_assumption :=
     |- _ => apply Henv in Hsem; [destruct Hsem |solve [auto]]; clear Henv
   end.
 
+
+Definition equiv_env (Is_free: ident -> Prop) R memories env menv :=
+  forall x c, Is_free x
+              -> sem_var_instant R x (present c)
+              -> (~PS.In x memories -> PM.find x env = Some c)
+              /\ (PS.In x memories -> mfind_mem x menv = Some c).
+
+Hint Unfold equiv_env.
+
+(* We often need to weaken an equivalence to a subterm: for example we
+know that the environments are equivalent for all [Is_free_caexp x
+(AnnExp e ck)], we can deduce that the environements are equivalent
+for all [Is_free_exp x e]. *)
+Lemma equiv_env_map (Is_free1 Is_free2: ident -> Prop) H memories env menv:
+  (forall x, Is_free2 x -> Is_free1 x) ->
+  equiv_env Is_free1 H memories env menv -> 
+  equiv_env Is_free2 H memories env menv.
+Proof.
+  intros Hinv Hequiv1 x **; auto.
+Qed.
+
+Ltac weaken_equiv_env :=
+  match goal with
+    | [H: equiv_env ?is_free1 ?R ?mems ?env ?menv 
+       |- equiv_env ?is_free2 ?R ?mems ?env ?menv] =>
+      eapply equiv_env_map; [|exact H]; constructor(auto)
+  end.
+
+
 Lemma clock_correct_true:
   forall R memories menv env ck,
-    (forall x c, Is_free_in_clock x ck
-                 -> sem_var_instant R x (present c)
-                 -> (~PS.In x memories -> PM.find x env = Some c)
-                    /\ (PS.In x memories -> mfind_mem x menv = Some c))
+    equiv_env (fun x => Is_free_in_clock x ck) R memories env menv
     -> sem_clock_instant R ck true
     -> Is_present_in memories menv env ck.
 Proof.
@@ -411,10 +437,7 @@ Qed.
 
 Lemma clock_correct_false:
   forall R memories menv env ck,
-    (forall x c, Is_free_in_clock x ck
-                 -> sem_var_instant R x (present c)
-                 -> (~PS.In x memories -> PM.find x env = Some c)
-                    /\ (PS.In x memories -> mfind_mem x menv = Some c))
+    equiv_env (fun x => Is_free_in_clock x ck) R memories env menv
     -> sem_clock_instant R ck false
     -> Is_absent_in memories menv env ck.
 Proof.
@@ -445,10 +468,7 @@ Qed.
 Lemma lexp_correct:
   forall R memories menv env c e,
     sem_lexp_instant R e (present c)
-    -> (forall x c, Is_free_in_lexp x e
-                    -> sem_var_instant R x (present c)
-                    -> (~PS.In x memories -> PM.find x env = Some c)
-                       /\ (PS.In x memories -> mfind_mem x menv = Some c))
+    -> equiv_env (fun x => Is_free_in_lexp x e) R memories env menv 
     -> exp_eval menv env (translate_lexp memories e) c.
 Proof.
   Hint Constructors exp_eval.
@@ -468,20 +488,14 @@ Qed.
 Lemma laexp_correct:
   forall R memories menv env c e,
     sem_laexp_instant R e (present c)
-    -> (forall x c, Is_free_in_laexp x e
-                    -> sem_var_instant R x (present c)
-                    -> (~PS.In x memories -> PM.find x env = Some c)
-                       /\ (PS.In x memories -> mfind_mem x menv = Some c))
+    -> equiv_env (fun x => Is_free_in_laexp x e) R memories env menv
     -> exp_eval menv env (translate_laexp memories e) c.
 Proof.
   intros H memories menv env c e Hsem Henv.
   destruct e as [ck ce].
   inversion Hsem as [? ? ? Hlexp|].
   change (exp_eval menv env (translate_lexp memories ce) c).
-  eapply lexp_correct; try eassumption.
-  intros; apply Henv.
-  + constructor (assumption). 
-  + assumption.
+  eapply lexp_correct; [eassumption | weaken_equiv_env]. 
 Qed.
 
 (** ** Validity of [translate_cexp] *)
@@ -489,10 +503,7 @@ Qed.
 Lemma cexp_correct:
   forall R memories prog menv env c x e,
     sem_cexp_instant R e (present c)
-    -> (forall x c, Is_free_in_cexp x e
-                    -> sem_var_instant R x (present c)
-                    -> (~PS.In x memories -> PM.find x env = Some c)
-                       /\ (PS.In x memories -> mfind_mem x menv = Some c))
+    -> equiv_env (fun x => Is_free_in_cexp x e) R memories env menv
     -> stmt_eval prog menv env (translate_cexp memories x e)
                                                         (menv, PM.add x c env).
 Proof.
@@ -521,10 +532,7 @@ Qed.
 Lemma caexp_correct:
   forall R memories prog menv env c x e,
     sem_caexp_instant R e (present c)
-    -> (forall x c, Is_free_in_caexp x e
-                    -> sem_var_instant R x (present c)
-                    -> (~PS.In x memories -> PM.find x env = Some c)
-                       /\ (PS.In x memories -> mfind_mem x menv = Some c))
+    -> equiv_env (fun x => Is_free_in_caexp x e) R memories env menv
     -> stmt_eval prog menv env (translate_caexp memories x e)
                                                   (menv, PM.add x c env).
 Proof.
@@ -552,23 +560,20 @@ Qed.
 
 (** ** More technical lemma! *)
 
-Lemma find_node_translate_find_class:
-  forall f G node,
-    find_node f G = Some node
-    -> (exists prog',
-           find_class f (translate G) = Some (translate_node node, prog')).
-Proof.
-  induction G as [|nd G IH]; [now inversion 1|].
-  intros node Hfind.
-  simpl; simpl in Hfind.
-  destruct (ident_eqb nd.(n_name) f) eqn:Heq.
-  - injection Hfind; intro He; rewrite He in *; clear He Hfind.
-    exists (translate G); reflexivity.
-  - apply IH in Hfind.
-    destruct Hfind as [prog'].
-    exists prog'.
-    assumption.
-Qed.
+Definition equiv_node G prog f :=
+  forall n xs ys M menv input output,
+    Memory_Corres G n f M menv 
+    -> msem_node G f xs M ys
+    -> xs n = present input 
+    -> ys n = present output 
+    -> exists menv',
+         stmt_step_eval prog menv f input menv' output 
+     /\  Memory_Corres G (S n) f M menv'.
+
+Definition equiv_prog G prog :=
+  forall f,
+    equiv_node G prog f.
+
 
 Lemma Is_memory_in_msem_var:
   forall G H M n x eqs c,
@@ -604,28 +609,29 @@ Qed.
 
 (** ** Validity of [translate_eqns] *)
 
+Section IsStepCorrect.
+
+Variables (G: global)
+          (HG: Welldef_global G)
+          (H: history)
+          (M: memory)
+          (mems: PS.t)
+          (alleqs : list equation)
+          (Hsems: msem_equations G H M alleqs)
+          (prog: program)
+          (input: ident).
+
+
 Lemma is_step_correct:
-  forall (G: global)
-         (H: history)
-         (M: memory)
-         (mems: PS.t)
-         (alleqs : list equation),
-
-    List.Forall (msem_equation G H M) alleqs
-
-    -> forall (prog: program)
-              (input: ident)
-              (eqs: list equation)
-              (n: nat)
-              (menv: heap)
-              (env: stack),
+  forall (eqs: list equation)
+         (n: nat)
+         (menv: heap)
+         (env: stack),
         (exists oeqs, alleqs = oeqs ++ eqs)
         -> (forall x, PS.In x mems
                       -> (Is_defined_in x alleqs
                           /\ ~Is_variable_in x alleqs))
-        -> Welldef_global G
-        -> prog = translate G
-
+        
         (* - input (assumed) *)
         -> (forall c, sem_var_instant (restr H n) input (present c)
                       <-> PM.find input env = Some c)
@@ -648,20 +654,7 @@ Lemma is_step_correct:
         -> Is_well_sch mems input eqs
 
         (* - instantiated nodes (assumed) *)
-        -> (forall f fnode xs M ys prog' fclass menv env,
-               find_node f G = Some fnode
-               -> msem_node G f xs M ys
-               -> Memory_Corres G n f M menv
-               -> find_class f prog = Some (fclass, prog')
-               -> env = match xs n with
-                        | absent => sempty
-                        | present c => PM.add (c_input fclass) c sempty
-                        end
-               -> exists menv' env',
-                   stmt_eval prog' menv env (c_step fclass) (menv', env')
-                   /\ (forall c, ys n = present c
-                                 <-> PM.find (c_output fclass) env' = Some c)
-                   /\ Memory_Corres G (S n) f M menv')
+        -> equiv_prog G prog
 
         (* - unwritten memories (assumed) *)
         -> List.Forall (Memory_Corres_eq G n M menv) alleqs
@@ -675,9 +668,6 @@ Lemma is_step_correct:
                (* - written memories (shown) *)
                /\ List.Forall (Memory_Corres_eq G (S n) M menv') eqs).
 Proof.
-  intros until alleqs.
-  intros Hsems.
-
   (* Induction on equations: translate_eqns [] = Skip *)
   induction eqs as [|eq];
     [ intros; exists menv, env;
@@ -685,7 +675,7 @@ Proof.
       split; intros; [ match goal with
                        | H:Is_variable_in _ nil |- _ => inversion H
                        end | now constructor ]| ].
-  intros n menv env Hall Hinmems Hwdef Hprog Hin Henv Hin1 Hin2 Hwsch Hnode Hmc.
+  intros n menv env Hall Hinmems Hin Henv Hin1 Hin2 Hwsch Hnode Hmc.
 
   assert (exists menv' env',
              stmt_eval prog menv env (translate_eqns mems eqs) (menv', env')
@@ -696,8 +686,6 @@ Proof.
   { eapply IHeqs.
     - apply List_shift_away with (1:=Hall).
     - exact Hinmems.
-    - exact Hwdef.
-    - exact Hprog.
     - exact Hin.
     - intros; apply Henv; constructor 2; auto.
     - exact Hin1.
@@ -725,11 +713,7 @@ Proof.
   - (* Case EqDef: y = cae *)
     exists menv'. (* the memory does not change *)
     specialize (Hcae n); simpl in *.
-    assert (forall x c, 
-               Is_free_in_caexp x cae
-            -> sem_var_instant (restr H n) x (present c)
-            -> (~ PS.In x mems -> PM.find x env' = Some c)
-               /\ (PS.In x mems -> mfind_mem x menv' = Some c))
+    assert (equiv_env (fun x => Is_free_in_caexp x cae) (restr H n) mems env' menv')
       as Hcae'. {
       intros. 
       split; intro Hmems.
@@ -825,11 +809,7 @@ Proof.
   - (* Case EqApp: y = f lae *)
     specialize (Hlae n).
     (* used variables are defined *)
-    assert (forall x c,
-               Is_free_in_laexp x lae
-               -> sem_var_instant (restr H n) x (present c)
-               -> (~ PS.In x mems -> PM.find x env' = Some c)
-                  /\ (PS.In x mems -> mfind_mem x menv' = Some c))
+    assert (equiv_env (fun x => Is_free_in_laexp x lae) (restr H n) mems env' menv')
       as Hlae'. {
       intros.
       split; intro Hmems.
@@ -919,33 +899,27 @@ Proof.
         rewrite stmt_eval_translate_eqns_minst_inv with (1:=Hstmt) (2:=Hniii).
         split; [exact Hfindo|].
         now apply Memory_Corres_unchanged
-        with (1:=Hwdef) (2:=Hmsem) (3:=Hls) (4:=Hmc0).
+        with (2:=Hmsem) (3:=Hls) (4:=Hmc0).
     + (* y = present *)
-      pose proof (find_node_translate_find_class _ _ _ Hfind) as Hfindc.
-      destruct Hfindc as [prog' Hfindc].
-      assert (
-          let fclass := translate_node (mk_node f i o neqs) in
-          exists omenv' oenv',
-            stmt_eval prog' omenv (PM.add i v sempty)
-                      (c_step fclass) (omenv', oenv')
-            /\ (forall c,
-                   xs n = present c
-                   <-> PM.find (c_output fclass) oenv' = Some c)
-            /\ Memory_Corres G (S n) f Mo omenv') as Hnode'.
-      { eapply Hnode with (1:=Hfind) (2:=Hmsem) (3:=Hmc0).
-        - rewrite Hprog; exact Hfindc.
-        - rewrite Hls; reflexivity. }
-      clear Hnode.
-      simpl in *.
-      destruct Hnode' as [omenv' [oenv' [Hnstmt [Hnout Hnmc]]]].
       assert (xs n <> absent) as Hxsp
           by (intro HH; apply Hout in HH; discriminate).
       apply not_absent_present in Hxsp.
       destruct Hxsp as [c Hxsc].
-      exists (madd_obj y omenv' menv'), (PM.add y c env').
+      rewrite Hxsc in *.
+
+      rename v into inValue. rename c into outValue.
+      
+      assert (exists menv' : heap,
+                stmt_step_eval prog omenv  f inValue menv' outValue
+             /\ Memory_Corres G (S n) f Mo menv') as Hclass
+             by (eapply Hnode; try eassumption).
+      destruct Hclass as [omenv' [Hnstmt Hnmc]].
+
+      simpl in *.
+      exists (madd_obj y omenv' menv'), (PM.add y outValue env'). 
       inversion Hlae as [? ? c0 Hlexp Hclk HR1 HR2|];
         rewrite <-HR1 in *; clear HR1 HR2 c0.
-      split; [|split].
+      split;[|split].
       * apply stmt_eval_translate_eqns_cons.
         exists menv', env'.
         split; [exact Hstmt|].
@@ -954,32 +928,25 @@ Proof.
         apply lexp_correct
         with (memories:=mems) (menv:=menv') (env:=env') in Hlexp;
           [|now auto].
-        rewrite Hprog in *.
         rewrite <-stmt_eval_translate_eqns_minst_inv
         with (1:=Hstmt) (2:=Hniii) in Hfindo.
-        eapply Istep with (1:=Hfindo) (2:=Hlexp);
-          [|reflexivity|reflexivity].
-        eapply Iestep with (1:=Hfindc) (2:=Hnstmt).
-        now apply Hnout with (1:=Hxsc).
-      * intros x Hivi c'.
-        inversion_clear Hivi as [? ? Hivi'|]; [inversion_clear Hivi'|].
-        { rewrite PM.gss; split; intro HH.
-          - assert ((xs n) = present c') by sem_det.
-            congruence.
-          - injection HH; intro Heq; rewrite <-Heq.
-            rewrite <-Hxsc; exact Hvar. }
-        { destruct (ident_eq_dec x y) as [Hxy|Hnxy].
-          - rewrite Hxy in *; clear Hxy.
-            rewrite PM.gss.
-            split.
-            * intro Hvar'.
-              assert (present c' = xs n) by sem_det.
+        eapply Istep; eauto.
+      * {
+          intros x Hivi c.
+          apply Is_variable_in_cons in Hivi.
+          destruct Hivi as [Hivi | [notxy Hivi] ].
+          - (* x = y *)
+            inversion_clear Hivi.
+            rewrite PM.gss. split; intro HH.
+            + assert (present c = present outValue) by sem_det.
               congruence.
-            * intro Hsv'.
-              injection Hsv'; intro Heq; rewrite <-Heq in *.
-              rewrite Hxsc in Hvar; exact Hvar.
-          - rewrite (PM.gso _ _ Hnxy).
-            apply IHeqs0; assumption. }
+            + injection HH. intro Heq; rewrite <-Heq.
+              apply Hvar.
+          - (* x <> y *)
+             not_Is_variable x y.
+             rewrite PM.gso; [|assumption].
+             apply IHeqs0; assumption.
+        }
       * apply Forall_cons.
         2:now apply Memory_Corres_eqs_add_obj with (1:=IHeqs1) (2:=Hniii).
         constructor.
@@ -990,11 +957,7 @@ Proof.
         split; [rewrite mfind_inst_gss; reflexivity|exact Hnmc].
   - (* Case EqFby: y = v0 fby lae *)
     specialize (Hlae n).
-    assert (forall x c,
-               Is_free_in_laexp x lae
-               -> sem_var_instant (restr H n) x (present c)
-               -> (~ PS.In x mems -> PM.find x env' = Some c)
-                  /\ (PS.In x mems -> mfind_mem x menv' = Some c))
+    assert (equiv_env (fun x => Is_free_in_laexp x lae) (restr H n) mems env' menv')
       as Hlae'. {
       intros.
       split; intro Hmems.
@@ -1090,152 +1053,156 @@ Proof.
         now apply mfind_mem_gss.
 Qed.
 
-(* TODO: rework using (a simplified version of) msem_node_mult *)
+End IsStepCorrect.
+
+Section IsNodeCorrect.
+
+
+Lemma equiv_prog_empty: equiv_prog [] (translate []).
+Proof.
+  intro Hwdef. 
+  intros n **.
+  exfalso.
+  repeat match goal with 
+      | H: msem_node [] _ _ _ _ |- _ => inversion H; clear H
+      | H: find_node _ [] = Some _ |- _ => inversion H; clear H
+         end.
+Qed.
+
 Lemma is_node_correct:
-  forall (G: global)
-         (f: ident)
-         (fnode: node)
-         (xs: stream value)
-         (M: memory)
-         (ys: stream value)
-
-         (prog': program)
-         (fclass: class)
-         (n: nat)
-         (menv: heap)
-         (env: stack),
-
-    Welldef_global G
-    -> find_node f G = Some fnode
-    -> msem_node G f xs M ys
-    -> Memory_Corres G n f M menv
-
-    -> find_class f (translate G) = Some(fclass, prog')
-    -> env = (match xs n with
-	      | present c => PM.add fclass.(c_input) c sempty
-	      | absent => sempty
-             end)
-
-    -> (exists menv' env',
-           stmt_eval prog' menv env fclass.(c_step) (menv', env')
-           /\ (forall c, ys n =present c
-                         <-> PM.find (fclass.(c_output)) env' = Some c)
-           /\ Memory_Corres G (S n) f M menv').
+  forall (G: global), 
+    Welldef_global G ->
+    equiv_prog G (translate G).
 Proof.
   (* TODO: Develop a version of msem_node_mult that works for eqs? *)
-  induction G as [|node G IH]; [now inversion 4|].
-  intros f fnode xs M ys prog' fclass n menv env.
-  intros Hwd Hfind Hmsem Hmc Hfcls Henv.
-  assert (Ordered_nodes (node::G)) as Hord
-      by apply Welldef_global_Ordered_nodes with (1:=Hwd).
+  induction G as [|node G IH].
+  - intro; apply equiv_prog_empty.
+  - intros Hwd f n xs ys M menv input output Hmc Hmsem Hxs Hys.
+    set (nodeName := n_name node).
 
-  simpl in Hfind,Hfcls.
-  destruct (ident_eqb (n_name node) f) eqn:Hfeq.
+    assert (Welldef_global G) as HwdG 
+        by (eapply Welldef_global_cons; eassumption).
 
-  Focus 2.
-  { apply Welldef_global_cons in Hwd.
-    assert (node.(n_name) <> f) as Hfneq
-        by apply Pos.eqb_neq with (1:=Hfeq).
-    rewrite Memory_Corres_node_tl with (1:=Hord) (2:=Hfneq) in Hmc.
-    apply msem_node_cons with (1:=Hord) (3:=Hfneq) in Hmsem.
-    apply IH with (1:=Hwd) (2:=Hfind) (3:=Hmsem) (4:=Hmc) (6:=Henv) (ys:=ys)
-      in Hfcls.
-    destruct Hfcls as [menv' [env' [Hstmt [Hout Hmc']]]].
-    exists menv',env'.
-    rewrite Memory_Corres_node_tl with (1:=Hord) (2:=Hfneq).
-    intuition. }
-  Unfocus.
+    assert (Ordered_nodes (node::G)) as Hord
+        by (apply Welldef_global_Ordered_nodes; assumption).
 
-  injection Hfcls; intros HR1 HR2; rewrite <-HR1,<-HR2 in *; clear HR1 HR2 Hfcls.
-  injection Hfind; intro HR1; rewrite HR1 in *; clear HR1 Hfind.
+    destruct (ident_eqb nodeName f) eqn:Hfeq.
+    + (* Case: f = nodeName *)
+      assert (nodeName = f)
+        by (apply Pos.eqb_eq; assumption). 
+      subst f.
+      
+      set (prog := translate (node :: G)).
 
-  inversion_clear Hmsem as [? ? ? ? i o eqs Hfind Hsem].
-  simpl in Hfind.
-  rewrite Hfeq in Hfind; clear Hfeq.
-  injection Hfind; intro HR1; rewrite HR1 in *; clear HR1 Hfind.
-  simpl in *.
+      inversion_clear Hwd as [|? ? Hwd' eqs inArg outArg 
+                               Hwsch Hndef_in Hdef_out Hnnode Hfind Hnodup].
+      clear Hwd'.
+      inversion_clear Hmsem as [? ? ? ? ? ? ? Heqs
+                                [H [Hin [Hout [Hrabs [Habs Hall]]]]]].
+      subst eqs inArg outArg nodeName.
+      simpl in Heqs; rewrite Hfeq in Heqs; simpl in Heqs.
+      injection Heqs. intro Hnode. rewrite Hnode in *. clear Heqs. simpl in *.
 
-  destruct Hsem as [H [Hi [Ho [Hclk [Hsout Hsem]]]]].
-  specialize (Hi n).
-  specialize (Ho n).
+      rename i into inArg; rename o into outArg; rename eqs0 into eqs.
 
-  inversion_clear Hwd as [|? ? Hwd' neqs ni no Hwsch Hin2 Hout Hnode Hnd Hfind'].
-  rename Hwd' into Hwd.
-  simpl in *.
-  unfold neqs, ni, no in *; clear neqs ni no.
+      set (env := PM.add inArg input sempty).
 
-  assert (
-      exists menv' env',
-        stmt_eval (translate G) menv env
-                  (translate_eqns (memories eqs) eqs) (menv', env')
-        /\ (forall x, Is_variable_in x eqs ->
-                     forall c, sem_var_instant (restr H n) x (present c)
-                               <-> PM.find x env' = Some c)
-        /\ Forall (Memory_Corres_eq G (S n) M menv') eqs) as His_step_correct.
-  {
-    eapply is_step_correct with (mems:=memories eqs) (env:=env) (menv:=menv)
-                                (input:=i) (prog:=translate G).
-    (* TODO: Tidy this up... *)
-    - apply Forall_msem_equation_global_tl
-      with (1:=Hord) (2:=Hnd) (3:=Hnode) (4:=Hsem).
-    - exists []; trivial.
-    - intros y Hinm.
-      assert (NoDup_defs eqs) as Hndds
-          by apply Is_well_sch_NoDup_defs with (1:=Hwsch).
-      split; [now apply Is_defined_in_memories with (1:=Hinm)
-             |now apply not_Is_variable_in_memories with (1:=Hinm) (2:=Hndds)].
-    - exact Hwd.
-    - reflexivity.
-    - intro c.
-      rewrite Henv.
-      split; intro HH.
-      assert (Hxs_pres: xs n = present c) by sem_det.
-      rewrite Hxs_pres in *.
-      apply PM.gss.
-      destruct (xs n) as [|v Hxs];
-        [ rewrite PM.gempty in HH; discriminate |].
-      rewrite PM.gss in HH; injection HH; intro HR1;
-      rewrite HR1 in *; exact Hi.
-    - rewrite Henv.
-      intros x Hivi.
-      destruct (xs n); [rewrite PM.gempty;reflexivity|].
-      rewrite PM.gso; [rewrite PM.gempty;reflexivity|].
-      apply Is_variable_in_Is_defined_in in Hivi.
-      intro Hx; rewrite Hx in *.
-      contradiction.
-    - intro Hin.
-      apply Is_defined_in_memories in Hin.
-      contradiction.
-    - exact Hin2.
-    - exact Hwsch.
-    - apply (fun f fnode xs M ys prog' fclass menv env Hfind Hmsem
-             => IH f fnode xs M ys prog' fclass n menv env Hwd Hfind Hmsem).
-    - inversion_clear Hmc as [? ? ? ? ? ? Hf Hmeqs].
-      simpl in Hf.
-      rewrite ident_eqb_refl in Hf.
-      injection Hf; intros Heq0 Heq1 Heq2;
-      rewrite <-Heq0, <-Heq1, <-Heq2 in *;
-      clear Heq0 Heq1 Heq2 Hf.
-      apply Memory_Corres_eqs_node_tl with (1:=Hord) (2:=Hnode) (3:=Hmeqs).
-  }
-  clear IH.
-  destruct His_step_correct as [menv' [env' [Hstmt [Hvar' Hmc']]]].
-  exists menv',env'.
-  split; [rewrite ps_from_list_gather_eqs_memories; exact Hstmt|].
-  split.
-  - intro c.
-    apply Hvar' with (c:=c) in Hout.
-    rewrite <- Hout.
-    split; intro HH;
-      [ rewrite HH in Ho; exact Ho 
-      | sem_det ].
-  - econstructor.
-    + simpl; rewrite Pos.eqb_refl; reflexivity.
-    + apply Memory_Corres_eqs_node_tl with (1:=Hord) (2:=Hnode) (3:=Hmc').
+      assert (msem_equations G H M eqs)
+        by (eapply Forall_msem_equation_global_tl; try eassumption).
+
+      assert (exists (menv' : heap) (env' : stack),
+                stmt_eval (translate G) menv env (translate_eqns (memories eqs) eqs) (menv', env') /\
+                (forall x : ident,
+                   Is_variable_in x eqs ->
+                   forall c : const,
+                     sem_var_instant (restr H n) x (present c) <->
+                     PM.find x env' = Some c) /\
+                Forall (Memory_Corres_eq G (S n) M menv') eqs) as His_step_correct.
+      {
+        eapply is_step_correct; try eassumption.
+        - exists []; auto.
+        - intros y Hinm.
+          assert (NoDup_defs eqs) as Hndds
+              by (eapply Is_well_sch_NoDup_defs; eauto).
+          split; [now apply Is_defined_in_memories
+                 |now apply not_Is_variable_in_memories].
+        - intro c.
+          specialize (Hin n); simpl in Hin.
+          split; intro HH.
+          + assert (Hxs_pres: c = input)
+              by (cut (xs n = present c);
+                  [ intro Hxsc; rewrite Hxsc in Hxs; injection Hxs; auto
+                  | sem_det]).
+            rewrite Hxs_pres in *.
+            subst env; apply PM.gss.
+          + subst env. rewrite PM.gss in HH. injection HH; intro HR1.
+            rewrite Hxs in Hin; rewrite HR1 in *. 
+            assumption.      
+        - intros x Hivi.
+          subst env.
+          rewrite PM.gso; [rewrite PM.gempty;reflexivity|].
+          apply Is_variable_in_Is_defined_in in Hivi.
+          intro Hx; rewrite Hx in *.
+          contradiction.
+        - intro HinArg.
+          apply Is_defined_in_memories in HinArg.
+          contradiction.
+        - eapply IH; assumption.
+        - inversion_clear Hmc as [? ? ? ? ? ? Hf Hmeqs].
+
+          simpl in Hf.
+          rewrite ident_eqb_refl in Hf.
+          injection Hf; intros Heq0 Heq1 Heq2;
+          rewrite <-Heq0, <-Heq1, <-Heq2 in *;
+          clear Heq0 Heq1 Heq2 Hf.
+          
+          eapply Memory_Corres_eqs_node_tl; try eassumption.
+      }
+
+      destruct His_step_correct as [menv' [env' [Hstmt [Hsemvar Hmem]]]].
+      exists menv'.
+      split.
+      * {
+          econstructor.
+          - simpl. rewrite Pos.eqb_refl. reflexivity.
+          - subst env. simpl.
+            assert (inArg = n_input node)
+              by (rewrite Hnode; auto).
+            assert (eqs = n_eqs node) 
+              by (rewrite Hnode; auto).
+            subst inArg; subst eqs.
+            rewrite ps_from_list_gather_eqs_memories. eapply Hstmt.
+          - assert (outArg = n_output node)
+              by (rewrite Hnode; auto).
+            subst outArg.
+            specialize (Hout n); simpl in Hout; rewrite Hys in Hout.
+            simpl. apply Hsemvar; try assumption.
+        }
+      * { 
+          econstructor.
+          - simpl; rewrite Pos.eqb_refl; reflexivity.
+          - eapply Memory_Corres_eqs_node_tl; eassumption.
+        }
+
+    + (* Case: f <> nodeName *)
+      assert (nodeName <> f) as Hfneq
+          by (eapply Pos.eqb_neq; try eassumption).
+
+      rewrite Memory_Corres_node_tl in Hmc; try eassumption.
+      apply msem_node_cons in Hmsem; try eassumption.
+      eapply IH in HwdG.
+      edestruct HwdG as [menv' [Hstmt' Hmc']]; try eassumption.
+      inversion_clear Hstmt'.
+      exists menv'; split.
+      * econstructor; try eassumption.
+        simpl; subst nodeName; rewrite Hfeq.
+        eassumption.
+      * rewrite Memory_Corres_node_tl; try assumption.
 Qed.
 
 (** ** Validity of the [reset] code *)
 
+(* TODO: remove after rewrite of translate_reset_eqns *)
 Lemma stmt_eval_translate_reset_eqn_shift:
   forall prog eqs iacc menv env menv' env',
     stmt_eval prog menv env
@@ -1324,134 +1291,174 @@ Qed.
    The case of EqFby is simpler due to the lemma Memory_Corres_eqs_add_mem.
    The comment following this lemma explains why there can be no corresponding
    Memory_Corres_eqs_add_obj lemma. *)
-Lemma is_node_reset_correct:
-  forall (G: global)
-         (f: ident)
-         (xs: stream value)
-         (M: memory)
-         (ys: stream value)
-         (fnode: node)
 
-         (prog': program)
-         (fclass: class)
-         (menv: heap)
-         (env: stack),
+Definition equiv_reset G prog f :=
+  forall xs ys M,
+    msem_node G f xs M ys 
+    -> exists menv',
+         stmt_reset_eval prog f menv'
+      /\ Memory_Corres G 0 f M menv'.
 
-       Welldef_global G
-    -> msem_node G f xs M ys
-    -> find_node f G = Some fnode
-
-    -> find_class f (translate G) = Some(fclass, prog')
-    -> (exists menv' env',
-           stmt_eval prog' hempty env fclass.(c_reset) (menv', env')
-           /\ Memory_Corres G 0 f M menv').
+(* TODO: remove/factorize with equiv_prog *)
+Lemma equiv_reset_empty: forall f, equiv_reset [] (translate []) f.
 Proof.
-  induction G as [|node G IH]; [now inversion 1|].
-  intros until env.
-  intros Hwdef Hmsem Hfindn Hfindc.
+  intro Hwdef. 
+  intros n **.
+  exfalso.
+  repeat match goal with 
+      | H: msem_node [] _ _ _ _ |- _ => inversion H; clear H
+      | H: find_node _ [] = Some _ |- _ => inversion H; clear H
+         end.
+Qed.
 
-  assert (Hfindn':=Hfindn).
-  pose proof (Welldef_global_Ordered_nodes _ Hwdef) as Hord.
-  pose proof (find_node_not_Is_node_in _ _ _ Hord Hfindn) as Hnni.
-  pose proof (find_node_translate_find_class _ _ _ Hfindn) as HH.
-  destruct HH as [prog'' Hfindc'].
-  rewrite Hfindc in Hfindc'.
-  injection Hfindc';
-    intros HR1 HR2; rewrite <-HR1,HR2 in *; clear HR1 HR2 Hfindc' prog''.
-  simpl in Hfindc, Hfindn'.
-  destruct (ident_eqb (n_name node) f) eqn:Heqb;
-    [ apply Pos.eqb_eq in Heqb | apply Pos.eqb_neq in Heqb ].
-  - injection Hfindn'; intro HR1; rewrite <-HR1 in *; clear HR1 Hfindn'.
-    injection Hfindc; intros HR1; rewrite <-HR1 in *; clear HR1 Hfindc.
-    destruct node as [f' i o eqs].
-    simpl in Heqb.
-    rewrite Heqb in *; clear Heqb.
-    cut (exists menv' env',
-            stmt_eval (translate G) hempty env (translate_reset_eqns eqs)
-                      (menv', env')
-            /\ Forall (Memory_Corres_eq G 0 M menv') eqs).
-    { destruct 1 as [menv' [env' [Hstmt Hmc]]].
+Section IsResetCorrect.
+
+Variables (G: global)
+          (HG: Welldef_global G)
+          (H: history)
+          (M: memory)
+          (mems: PS.t)
+          (input: ident).
+
+
+Lemma is_reset_correct:
+  forall eqs, 
+    msem_equations G H M eqs ->
+    Is_well_sch mems input eqs ->
+    (forall f, equiv_reset G (translate G) f) ->
+  exists menv' env',
+    stmt_eval (translate G) hempty sempty (translate_reset_eqns eqs)
+              (menv', env')
+    /\ Forall (Memory_Corres_eq G 0 M menv') eqs.
+Proof.
+  intros eqs Hmsem Hwsch Hreset.
+  induction eqs as [|eq eqs IH]; [eauto|].
+  destruct eq as [i e|i f e|i v e];
+  inversion_clear Hmsem as [| ? ? Hsem Hmsem' ];
+  inversion_clear Hwsch;
+  edestruct IH as [menv' [env' [Hstmt Hmc]]]; try eassumption.
+  - (* EqDef *)
+    Hint Constructors Forall.
+    Hint Constructors Memory_Corres_eq.
+    eauto.
+  - (* EqApp *)
+    unfold translate_reset_eqns; simpl.
+    inversion_clear Hsem as [|? ? ? ? Mo ? xs' ys' Hmfind Hxs' Hys' HsemNode|].
+    assert (exists omenv, stmt_reset_eval (translate G) f omenv 
+                       /\ Memory_Corres G 0 f Mo omenv) as [omenv [Hstmt_reset Hmcf]]
+      by (eapply Hreset; try eassumption).
+    
+    exists (madd_obj i omenv menv'), env'.
+    split.
+    + rewrite stmt_eval_translate_reset_eqn_shift.
       exists menv', env'.
-      split; [exact Hstmt|].
-      econstructor; [exact Hfindn|].
-      apply Memory_Corres_eqs_node_tl with (1:=Hord) (2:=Hnni).
-      exact Hmc. }
-    simpl in *.
-    inversion_clear Hmsem as [? ? ? ? i' o' eqs' Hfind HH].
-    simpl in Hfind; rewrite ident_eqb_refl in Hfind.
-    injection Hfind; intros HR1 HR2 HR3; rewrite <-HR1,<-HR2,<-HR3 in *;
-    clear HR1 HR2 HR3 Hfind f' i' o' eqs'.
-    destruct HH as [H [Hxs [Hys [Habs [Hout Hmsem]]]]].
-    apply Forall_msem_equation_global_tl with (1:=Hord) (3:=Hnni) in Hmsem.
-    2:(intros f' Hini'; apply find_node_Exists; inversion_clear Hord;
-       apply H1 in Hini'; now intuition).
-    clear Hxs Hys Habs Hout Hfindn Hord.
-    assert (exists mems, Is_well_sch mems i eqs) as Hwsch
-        by (inversion_clear Hwdef; exists (memories eqs0); intuition).
-    destruct Hwsch as [mems Hwsch].
-    apply Welldef_global_cons in Hwdef.
-    induction eqs as [|eq eqs IHeqs]; [exists hempty, env; now intuition|].
-    apply not_Is_node_in_cons in Hnni.
-    destruct Hnni as [Hnni Hnnis].
-    apply Forall_cons2 in Hmsem; destruct Hmsem as [Hmsem Hmsems].
-    specialize (IHeqs Hnnis Hmsems (Is_well_sch_cons _ _ _ _ Hwsch)); clear Hnnis.
-    destruct IHeqs as [menv' [env' [Hstmt Hmc]]].
-    rewrite stmt_eval_translate_reset_eqns_cons.
-    exists menv', env'.
-    destruct eq as [|y g lae|y v0 lae].
-    + (* EqDef *)
+      split; try assumption.
+      econstructor; [|constructor].
+      econstructor; auto.
+      assumption.
+    + repeat constructor; [| apply Memory_Corres_eqs_add_obj; assumption].
+      intros M' Hmfind'.
+      rewrite Hmfind in Hmfind'; injection Hmfind'; intro Heq; subst M'.
+      exists omenv.
+      rewrite mfind_inst_gss.
+      auto.
+  - (* EqFby *)
+    exists (madd_mem i v menv'), env'.
+    split.
+    + unfold translate_reset_eqns; simpl;
+        rewrite stmt_eval_translate_reset_eqn_shift.
       exists menv', env'.
-      split; [exact Hstmt|].
-      split; [constructor|].
-      inversion_clear Hwsch.
-      repeat constructor.
-      exact Hmc.
-    + (* EqApp *)
-      inversion_clear Hmsem as [|? ? ? ? Mo ? xs' ys' Hmfind Hxs' Hys' Hmsem'|].
-      assert (Hmsem'':=Hmsem').
-      inversion_clear Hmsem'' as [? ? ? ? ? ? ? Hfindn HH].
-      pose proof (find_node_translate_find_class _ _ _ Hfindn) as Hfindc.
-      destruct Hfindc as [prog'' Hfindc].
-      specialize (IH _ _ _ _ _ _ _ hempty sempty Hwdef Hmsem' Hfindn Hfindc).
-      destruct IH as [omenv [oenv [Hstmtn Hmcn]]].
-      exists (madd_obj y omenv menv'), env'.
-      split; [exact Hstmt|].
+      Hint Constructors stmt_eval.
+      eauto.
+    + inversion_clear Hsem as [| | ? ? ? ? ? ? ? ? Hmfind Hms Hlae Hls]. 
+      rewrite <- Hms.
+      constructor; [|apply Memory_Corres_eqs_add_mem; assumption].
+      constructor. intros ms' Hmfind'.
+      rewrite Hmfind in Hmfind'.
+      injection Hmfind'; intro HR; rewrite HR in *; clear HR Hmfind'.
+      rewrite mfind_mem_gss.
+      reflexivity.
+Qed.
+
+End IsResetCorrect.
+
+Lemma is_node_reset_correct:
+  forall (G: global) f,
+         Welldef_global G ->
+         equiv_reset G (translate G) f.
+Proof.
+  induction G as [|node G IH].
+  - intros f Hwd.
+    apply equiv_reset_empty.
+  - intros f Hwdef xs ys M Hmsem.
+
+    assert (Ordered_nodes (node :: G)) as HordG
+      by (apply Welldef_global_Ordered_nodes; assumption).
+    
+    set (nodeName := n_name node).
+
+    destruct (ident_eqb nodeName f) eqn:Heqb.
+    + assert (nodeName = f) as Hfeq 
+        by (apply Pos.eqb_eq; assumption).
+
+      inversion_clear Hmsem as [? ? ? ? inArg outArg eqs Hfind 
+                                [H [Hin [Hout [Hrhs [Habs Hmsem']]]]]].
+      rename Hmsem' into Hmsem.
+
+      specialize (Hin 0)%nat; specialize (Hout 0)%nat;
+        simpl in Hin, Hout.
+
+      simpl in Hfind; subst nodeName; rewrite Heqb in Hfind; 
+      injection Hfind; clear Hfind; intro Hfind. 
+
+      assert (msem_equations G H M eqs).
+      {
+        inversion_clear Hwdef. subst eqs0; rewrite Hfind in *; simpl in *.
+        eapply Forall_msem_equation_global_tl; try eassumption.
+      }
+
+      assert (Is_well_sch (memories eqs) inArg eqs)
+        by (inversion Hwdef; subst ni eqs0;
+            rewrite Hfind in *; simpl in *; assumption).
+
+      assert (Welldef_global G) 
+        by (inversion Hwdef; assumption).
+
+      assert (exists menv' env',
+             stmt_eval (translate G) hempty sempty (translate_reset_eqns eqs)
+                       (menv', env')
+             /\ Forall (Memory_Corres_eq G 0 M menv') eqs) 
+        as [menv' [env' [Hstmt Hmc]]].
+      {
+        eapply is_reset_correct; try eassumption.
+        intro; apply IH; assumption.
+      }
+      
+      exists menv'.
       split.
-      * econstructor; [|now econstructor].
-        econstructor; [|reflexivity].
-        econstructor; [exact Hfindc|].
-        exact Hstmtn.
-      * inversion_clear Hwsch.
-        repeat constructor;
-          [|apply Memory_Corres_eqs_add_obj with (1:=Hmc); assumption].
-        intros M' Hmfind'.
-        rewrite Hmfind in Hmfind'.
-        injection Hmfind'; intro HR; rewrite <-HR; clear HR Hmfind' M'.
-        exists omenv.
-        split; [now apply mfind_inst_gss|now intuition].
-    + (* EqFby *)
-      exists (madd_mem y v0 menv'), env'.
-      split; [exact Hstmt|].
-      split.
-      * econstructor; [|now econstructor].
-        econstructor; [|reflexivity].
-        now constructor.
-      * inversion_clear Hmsem as [| |? ? ? ? ? ? ? ? Hmfind Hms Hlae Hls].
-        rewrite <-Hms in *.
-        repeat constructor;
-          [| now apply Memory_Corres_eqs_add_mem with (1:=Hmfind) (2:=Hmc)].
-        intros ms' Hmfind'.
-        rewrite Hmfind in Hmfind'.
-        injection Hmfind'; intro HR; rewrite HR in *; clear HR Hmfind'.
-        rewrite mfind_mem_gss.
-        reflexivity.
-  - apply Welldef_global_cons in Hwdef.
-    apply msem_node_cons with (1:=Hord) (3:=Heqb) in Hmsem.
-    specialize (IH _ _ _ _ _ _ _ menv env Hwdef Hmsem Hfindn' Hfindc).
-    destruct IH as [menv' [env' [Hstmt Hmc]]].
-    exists menv', env'.
-    split; [exact Hstmt|].
-    now apply Memory_Corres_node_tl with (1:=Hord) (2:=Heqb) (3:=Hmc).
+      * { 
+          econstructor. 
+          - simpl. rewrite Heqb. reflexivity.
+          - subst node; eassumption.
+        }
+      * { 
+          econstructor.
+          - simpl; rewrite Heqb. subst node. reflexivity.
+          - apply Memory_Corres_eqs_node_tl; try assumption.
+            inversion Hwdef. subst eqs0. rewrite Hfind in *. simpl. assumption.
+        }
+
+    + assert (nodeName <> f) as Hfneq
+        by (apply Pos.eqb_neq; assumption).
+
+      apply Welldef_global_cons in Hwdef.
+      apply msem_node_cons in Hmsem; try assumption.
+      edestruct IH as [menv' [Hstmt Hmc]]; try eassumption.
+      exists menv'; split.
+      * inversion_clear Hstmt.
+        econstructor; try eassumption.
+        simpl. subst nodeName; rewrite Heqb. assumption.
+      * apply Memory_Corres_node_tl; eassumption.
 Qed.
 
 (** ** Validity of the whole translation *)
@@ -1474,8 +1481,6 @@ Lemma is_translate_correct:
                    (Repeat (S n) (Step_ap r f obj (Const ci)))) (menv, env)
            /\ (forall co, ys n = present co <-> PM.find r env = Some co)).
 Proof.
-  (* TODO: Ugly, dumb proof. How to streamline / beautify all these
-           inversions and rewrites. *)
   intros until n.
   intros Hwdef Hsem Hxs.
   apply sem_msem_node with (1:=Hwdef) in Hsem.
@@ -1483,128 +1488,63 @@ Proof.
   assert(Hmsem':=Hmsem).
   inversion_clear Hmsem' as [? ? ? ? ? ? ? Hfindn Hmsem''].
   destruct Hmsem'' as [H [Hi [Ho [Hclk [Habs Hmsem']]]]].
-  pose proof (find_node_translate_find_class _ _ _ Hfindn) as Hfindc.
-  destruct Hfindc as [prog' Hfindc].
-  pose proof (is_node_reset_correct _ _ _ _ _ _ _ _
-                                    hempty sempty Hwdef Hmsem Hfindn Hfindc) as Hreset.
-  destruct Hreset as [menv' [env' [Hstmtr Hmc0]]].
-  simpl in Hstmtr.
-  cut (exists menv env,
-          stmt_eval (translate G) hempty sempty
-                    (Comp (Reset_ap f obj) (Repeat (S n)
-                                               (Step_ap r f obj (Const ci))))
-                    (menv, env)
-          /\ (forall co, ys n = present co <-> PM.find r env = Some co)
-          /\ (exists omenv, mfind_inst obj menv = Some omenv
-                            /\ Memory_Corres G (S n) f M omenv)).
-  destruct 1 as [menv [env [Hstmt [Hout Hmc]]]]; exists menv, env; now intuition.
-  induction n.
-  - specialize Hxs with 0%nat.
-    pose proof (is_node_correct _ _ _ _ _ _ _ _ _ _ (PM.add i ci sempty)
-                                Hwdef Hfindn Hmsem Hmc0 Hfindc) as Hstmt.
-    rewrite Hxs in Hstmt; specialize (Hstmt (eq_refl _)); simpl in Hstmt.
-    destruct Hstmt as [menv'' [env'' [Hstmt [Hout Hmc]]]].
-    assert (ys 0%nat <> absent) as Hyna
-        by (intro HH; apply Habs in HH; rewrite Hxs in HH; discriminate).
-    apply not_absent_present in Hyna.
-    destruct Hyna as [yc Hyna].
-    exists (madd_obj obj menv'' (madd_obj obj menv' hempty)).
-    exists (PM.add r yc sempty).
-    split; [|split].
-    + (* TODO: automate! *)
-      econstructor.
-      econstructor; [|reflexivity].
-      econstructor; [exact Hfindc|exact Hstmtr].
-      econstructor.
-      econstructor.
-      econstructor.
-      apply mfind_inst_gss.
-      econstructor.
-      econstructor.
-      exact Hfindc.
-      apply Hstmt.
-      apply Hout.
-      apply Hyna.
-      reflexivity.
-      reflexivity.
-    + (* TODO: automate *)
-      intuition.
-      rewrite H0 in Hyna.
-      injection Hyna; intro; subst.
-      apply PM.gss.
-      rewrite PM.gss in H0.
-      injection H0; intro; subst.
-      exact Hyna.
-    + exists menv''.
-      intuition.
-      apply mfind_inst_gss.
-  - destruct IHn as [menv'' [env'' [Hstmts [H0 Hmc]]]]; clear H0.
-    destruct Hmc as [omenv [Hfindo Hmc]].
-    inversion_clear Hstmts.
-    specialize Hxs with (S n).
-    pose proof (is_node_correct _ _ _ _ _ _ _ _ _ _ (PM.add i ci sempty)
-                                Hwdef Hfindn Hmsem Hmc Hfindc) as Hstmt.
-    rewrite Hxs in Hstmt; specialize (Hstmt (eq_refl _)); simpl in Hstmt.
-    destruct Hstmt as [menv''' [env''' [Hstmt [Hout Hmc']]]].
-    assert (ys (S n) <> absent) as Hyna
-        by (intro HH; apply Habs in HH; rewrite Hxs in HH; discriminate).
-    apply not_absent_present in Hyna.
-    destruct Hyna as [yc Hyna].
-    exists (madd_obj obj menv''' menv'').
-    exists (PM.add r yc env'').
-    split; [|split].
-    + (* TODO: automate! *)
-      econstructor.
-      exact H0.
-      econstructor.
-      exact H1.
-      econstructor.
-      exact Hfindo.
-      econstructor.
-      econstructor.
-      exact Hfindc.
-      apply Hstmt.
-      apply Hout.
-      apply Hyna.
-      reflexivity.
-      reflexivity.
-    + (* TODO: automate! *)
-      intuition.
-      rewrite H2 in Hyna.
-      injection Hyna; intro; subst.
-      apply PM.gss.
-      rewrite PM.gss in H2.
-      injection H2; intro; subst.
-      exact Hyna.
-    + exists menv'''.
-      intuition.
-      apply mfind_inst_gss.
-Qed.
 
-Lemma is_translate_even_more_correct:
-  forall (G: global)
-         (f: ident)
-         (xs: stream value)
-         (ys: stream value)
-         (ci: const)
-         (r: ident)
-         (obj: ident)
-         (n: nat)
-         (menv: heap)
-         (env: stack),
-    Welldef_global G
-    -> sem_node G f xs ys
-    -> (forall n, xs n = present ci)
-    -> stmt_eval (translate G) hempty sempty
-                 (Comp (Reset_ap f obj)
-                       (Repeat (S n) (Step_ap r f obj (Const ci)))) (menv, env)
-    -> (forall co, ys n = present co <-> PM.find r env = Some co).
-Proof.
-  intros G f xs ys ci r obj n menv env Hwdef Hsem Hin Hstmt.
-  pose proof (is_translate_correct G f xs ys ci r obj n Hwdef Hsem Hin) as Hc.
-  destruct Hc as [menv2 [env2 [Hstmt2 Hout]]].
-  apply stmt_eval_det with (1:=Hstmt) in Hstmt2.
-  injection Hstmt2; intros; subst.
-  now apply Hout.
+  assert (exists menv0,
+            stmt_reset_eval (translate G) f menv0
+         /\ Memory_Corres G 0 f M menv0) as [menv0 [Hstmtr Hmc0]]
+      by (eapply is_node_reset_correct; try eassumption).
+
+  (* TODO: extract as a standalone lemma *)
+  assert (forall n, 
+          exists menvN omenvN envN,
+            stmt_eval (translate G) (madd_obj obj menv0 hempty) sempty
+                      (Repeat (S n) (Step_ap r f obj (Const ci)))
+                      (menvN, envN)
+            /\ mfind_inst obj menvN = Some omenvN
+            /\ Memory_Corres G (S n) f M omenvN
+            /\ (forall co, ys n = present co <-> PM.find r envN = Some co)).
+  {
+
+    induction 0.
+    - specialize Hxs with 0%nat.
+
+      assert (exists co0, ys 0 = present co0)%nat as [co0 Hco0]
+             by (apply not_absent_present; rewrite <- Habs; congruence).
+
+      assert (exists menv,
+              stmt_step_eval (translate G) menv0 f ci menv co0
+              /\  Memory_Corres G 1 f M menv) as [menv1 [Hstmt1 Hmem1]]
+        by (eapply is_node_correct; try eassumption).
+
+      do 3 eexists.
+      split; [|split; [| split]]; try eauto.
+      + econstructor; [econstructor|].
+        econstructor; try eauto.        
+        apply mfind_inst_gss.
+      + apply mfind_inst_gss.
+      + rewrite Hco0, PM.gss. intuition; congruence.
+
+    - destruct IHn0 as [menv' [omenv' [env' [Hstmt [Hfind [Hmc _]]]]]].
+
+      assert (exists coSn, ys (S n0) = present coSn) as [coSn Hys] 
+          by (apply not_absent_present; rewrite <- Habs; congruence).
+
+      assert (exists omenv'',
+                stmt_step_eval (translate G) omenv' f ci omenv'' coSn
+            /\  Memory_Corres G (S (S n0)) f M omenv'') as [omenvSn [HstmtSn HmemSn]]
+        by (specialize Hxs with (S n0); eapply is_node_correct; try eassumption).
+
+      do 3 eexists. 
+      split; [|split; [| split]]; try eauto.
+      + rewrite mfind_inst_gss; auto.
+      + rewrite Hys, PM.gss. intuition; congruence.
+  }
+
+  edestruct H0 as [menv [omenv [env [Hstmt [Hfind [Hmc Hpres]]]]]].
+
+  exists menv, env.
+  split; try eassumption.
+  econstructor; try eassumption.
+  econstructor; try eauto.
 Qed.
 
