Translation.v
@@ -103,6 +103,7 @@ Definition translate_reset_eqn (s: stmt) (eqn: equation): stmt :=
 Definition ps_from_list (l: list ident) : PS.t :=
   List.fold_left (fun s i=>PS.add i s) l PS.empty.
 
+(* TODO: remove CPS in translate_reset_eqn *)
 Definition translate_reset_eqns (eqns: list equation): stmt :=
   List.fold_left translate_reset_eqn eqns Skip.
 
